compiler/core/Compiler/Enhanced/EnhancedDataToEJson.v
@@ -34,7 +34,7 @@ Import ListNotations.
 Local Open Scope list_scope.
 
 Program Instance enhanced_foreign_to_ejson : foreign_to_ejson :=
-  mk_foreign_to_ejson enhanced_foreign_runtime enhanced_foreign_ejson _ _ _ _.
+  mk_foreign_to_ejson enhanced_foreign_runtime enhanced_ejson enhanced_foreign_ejson _ _ _ _.
 Next Obligation.
   exact j. (* XXX enhanced_ejson is the same as enhanced_data *)
 Defined.
@@ -121,8 +121,9 @@ Qed.
 
 Program Instance enhanced_foreign_to_ejson_runtime : foreign_to_ejson_runtime :=
   mk_foreign_to_ejson_runtime
-    enhanced_foreign_runtime
+    enhanced_ejson
     enhanced_foreign_ejson
+    enhanced_foreign_runtime
     enhanced_foreign_to_ejson
     enhanced_foreign_ejson_runtime
     _ _ _ _ _ _.
